Invariant/ValidAttacker/ValidAttackerIII/OneStepPreservesValidAttackerIII.v
@@ -13,6 +13,9 @@ Require Import Invariant.AuxLemmas.AuxLemmas.
 Require Import Invariant.AuxTactics.
 
 Require Import Invariant.ValidAttacker.ValidAttackerIII.RemoteServices.
+Require Import Invariant.ValidAttacker.ValidAttackerIII.ExploitationRemoteServices.
+Require Import Invariant.ValidAttacker.ValidAttackerIII.RemoteSystemDiscovery.
+Require Import Invariant.ValidAttacker.ValidAttackerIII.SystemServiceDiscovery.
 
 Theorem one_step_preserves_valid_attacker_iii : forall (a a' : Attacker) (t : Technique) (n: network_map),
       one_step a t n a' -> valid_attacker_iii a'.
@@ -22,4 +25,15 @@ Theorem one_step_preserves_valid_attacker_iii : forall (a a' : Attacker) (t : Te
     induction t; unfold valid_attacker in H0; unfold valid_concrete_network in H;
     unfold Pre in H1; unfold Post in H2; unfold valid_attacker_iii.
     - apply (one_step_remote_services_preserves_valid_attacker_iii a a' network H0 i i1 i0 i2 k i3); auto.
+    - apply (one_step_exploitation_remote_services_preserves_valid_attacker_iii a a' network H0 i i1 i0 i2 i3); auto.
+    - admit. (* Unsecured_Credentials *)
+    - admit. (* Brute_Force *)
+    - admit. (* Abuse_Elevation_Control_Mechanism *)
+    - admit. (* File_Directory_Discovery_Local *)
+    - admit. (* File_Directory_Discovery_Remote *)
+    - admit. (* Network_Service_Scanning *)
+    - apply (one_step_remote_system_discovery_preserves_valid_attacker_iii a a' network H0 i i0); auto.
+    - admit. (* Account_Discovery_Local *)
+    - admit. (* Account_Discovery_Remote *)
+    - apply (one_step_system_service_discovery_preserves_valid_attacker_iii a a' network H0 i i0); auto.
   Admitted.
